\newpage
\section{Derivations}

\subsection{Derivation for \Section{split}}
\label{app:proof-kalman}
Let us consider the Kalman Filter measurement update equations introduced in Table \Table{ekalman}, recalling to the reader that we are considering the case in which the measurement $z_n = x_n^*$ is in the same space of the estimated state $\hat{x}_n$, thus when $J$ is the identity matrix.
% 
\begin{align*}
\hat{x}_n 
&= \hat{x}_n^0 + P_n^0  (P_n^0 + R)^{-1}(z_n - \hat{x}_n^0) \\
&= (P_n^0 + R)(P_n^0 + R)^{-1}\hat{x}_n^0 + P_n^0  (P_n^0 + R)^{-1}(z_n - \hat{x}_n^0) \\
&= R(P_n^0 + R)^{-1}\hat{x}_n^0 + P_n^0  (P_n^0 + R)^{-1}z_n \\
% 
% 
P_n &= ((P_n^0 + R) (P_n^0 + R)^{-1} - P_n^0  (P_n^0 + R)^{-1}) P_n^0\\
&= R (P_n^0 + R)^{-1} P_n^0
\end{align*}
% 
Note how these two coincide with \Equation{combining} for product of two Gaussians  with $z_n = x_n^*$, $P_n^0 = \hat{\Sigma}_{n - 1}$ and $R = \Sigma_{n}$.

\subsection{Derivation for \Section{joint}}
\label{app:ieif-lm}
%
To show that the optimizing the objective in Table \Table{iekf-like} with Levenberg-Marquardt (LM) is equivalent to an IEKF, we first convert the EKF into an EIF like the one of \Appendix{eif}. Then, similarly to \Appendix{iekf}, we can write the iterated version of an EIF, as reported in \Table{ieif}. The LM update in the optimization associated to Table \ref{tab:iekf-like} then can be written as:
% 
\begin{equation}
    x_n^{i + 1}= x_n^{i} - (\bar{J}_n^T \bar{J}_n)^{-1} \bar{J}_n^T \bar{F}_n 
\end{equation}
 with $\bar{J}_n$ and $\bar{F}_n$ expanded below, $F_n^i = F(x_n^i)$, 
 $J_n^i = \frac{\partial F}{\partial x_n}(x_n^i)$, the measurement $z_n = d_n$ and $\hat{\Sigma}_n^{-1} = r H_{n - 1}$. 
 
 \begin{align*}
x_n^{i + 1}= x_n^{i} - \left(
\left[
	\begin{array}{cc}
		- J_n^i \\
		\left(r H_{n - 1}\right)^{1/2} \\
	\end{array}
\right]^T 
\left[
	\begin{array}{c}
		- J_n^i \\
		\left(r H_{n - 1}\right)^{1/2} \\
	\end{array}
\right]
\right)^{-1} \times\\
\times \left[
	\begin{array}{cc}
		- J_n^i \\
		\left(r H_{n - 1}\right)^{1/2} \\
	\end{array}
\right]^T 
\left[
	\begin{array}{c}
		z_n - F_n^i \\
		\left(r H_{n - 1}\right)^{1/2}(x_n^i - \hat{x}_{n - 1}) \\
	\end{array}
\right] = \\
= x_n^{i} - \underbrace{\left({J_n^i}^T J_n^i + r H_{n - 1}\right)^{-1}}_{A} \times \\
\times \left( - {J_n^i}^T(z_n - F_n^i) + r H_{n - 1}(x_n^i - \hat{x}_{n - 1})\right)  = \\
= x_n^i +\underbrace{A {J_n^i}^T(z_n - F_n^i)}_B - A r H_{n - 1}(x_n^i - \hat{x}_{n - 1})  = \\
= \hat{x}_{n - 1} + B  - A r H_{n - 1}(x_n^i - \hat{x}_{n - 1}) + A A^{-1}( x_n^i - \hat{x}_{n - 1}) = \\
= \hat{x}_{n - 1} + B + A(- r H_{n - 1} + {J_n^i}^T J_n^i + r H_{n - 1})(x_n^i - \hat{x}_{n - 1}) = \\
= \hat{x}_{n - 1} + B + A {J_n^i}^T J_n^i (x_n^i - \hat{x}_{n - 1}) = \\
= \hat{x}_{n - 1} + \underbrace{\left({J_n^i}^T J_n^i + r H_{n - 1}\right)^{-1} {J_n^i}^T}_{K_n^i}  \big(z_n - F_n^i - J_n^i (\hat{x}_{n - 1} - x_n^i)\big),
\end{align*}
% 
which is equivalent to the measurement update of IEIF from Table \ref{tab:ieif}, with $H_n^0 = H_{n-1}$ and $x_n^0 = \hat{x}_{n - 1}$.
\input{tab/ieif.tex}
\TODO{ where $\times$ denotes the standard matrix product.}
% \input{fig/merging/item}